LeanProofs/LeanProofs.lean
@@ -2,4 +2,4 @@
 -- Import modules here that should be built as part of the library.
 import LeanProofs.Basic
 import LeanProofs.Hash
-import LeanProofs.exprDeterminism
+import LeanProofs.stateEquivalence
